kernel/cemitcodes.ml
@@ -258,6 +258,9 @@ let emit_instr = function
   | Kareconst(n,lbl) -> out opARECONST; out_int n; out_label lbl
   | Kcompint31 -> out opCOMPINT31
   | Kdecompint31 -> out opDECOMPINT31
+  | Klorint31 -> out opORINT31
+  | Klandint31 -> out opANDINT31
+  | Klxorint31 -> out opXORINT31
   (*/spiwack *)
   | Kstop ->
       out opSTOP
